####
# Athlinks Ontology
# Version: 1.0-3.2
# Includes owlized version of http://schema.org version 3.2
####

@prefix : <http://adp.athlinks.com/schema/> .
@prefix dc: <http://purl.org/dc/elements/1.1/> .
@prefix owl: <http://www.w3.org/2002/07/owl#> .
@prefix rdf: <http://www.w3.org/1999/02/22-rdf-syntax-ns#> .
@prefix xml: <http://www.w3.org/XML/1998/namespace> .
@prefix xsd: <http://www.w3.org/2001/XMLSchema#> .
@prefix rdfs: <http://www.w3.org/2000/01/rdf-schema#> .
@prefix schema: <http://schema.org/> .

: a owl:Ontology ;
	owl:versionIRI <http://adp.athlinks.com/schema/1.0-3.2/> ;
  # import our owlized version of schema.org
	owl:imports <http://adp.athlinks.com/schemax/> ;
	rdfs:comment "This file contains Athlinks data vocabulary. The vocabulary is based on the schema.org ontology with our own extensions for concepts specific to human endurance events."@en ;
	rdfs:label "Athlinks data vocabulary"@en ;
	dc:contributor "astn" , 
                 "nextdude" , 
                 "warren" ,
                 "berg" .

####
# Properties
####
:eventAction a owl:ObjectProperty ;
        rdfs:subPropertyOf schema:item ;
        rdfs:domain :AthleteResult ;
        rdfs:range :AthleticEventAction ;
        rdfs:comment "A pointer to the the athletic event action that is being ranked."@en ;
        rdfs:label "event action"@en .

:legacyData a owl:ObjectProperty ;
	rdfs:domain owl:Thing ;
	rdfs:range :LegacyDataRole ;
	rdfs:comment "A legacy data record belonging to another system that is related to this object."@en ;
	rdfs:label "legacy data"@en .

# TODO: This shouldn't be defined on schema:Person. It should be computed by query.
# Or available in racer metrics. - nextdude
:participatedIn a owl:ObjectProperty ;
	rdfs:domain schema:Person ;
  rdfs:range :AthleticEventCategory ;
	rdfs:comment "An indication of a person participating in an event category."@en ;
	rdfs:label "participated in"@en .

# virtual property - computed on the fly by the api
:age a owl:DatatypeProperty ;
	rdfs:domain schema:Person ;
	rdfs:range xsd:integer ;
	rdfs:comment "The age (in years) of a person. Note that we don't store this constantly changing value in our database, but rather compute it dynamically when queried based on schema:birthDate."@en ;
	rdfs:label "age"@en .

:athleteCohort a owl:ObjectProperty ;
  rdfs:domain [
    rdf:type owl:Class;
    owl:unionOf (
      :AthleteResult
      :AthleteResultList
    );
  ];
  rdfs:range :AthleteCohort ;
  rdfs:comment "The athlete cohort to which a result or result list belongs."@en ;
  rdfs:label "athlete cohort"@en .

:rank a owl:DatatypeProperty ;
	rdfs:subPropertyOf schema:position ;
	rdfs:domain :AthleteResult ;
	rdfs:range [
          rdf:type owl:Class;
          owl:unionOf (
            xsd:integer
            xsd:string
          );
        ];
  rdfs:comment "Rank of a course time result in the context of a particular athlete cohort. The rank may differ from its [position](http://schema.org/position), which is assumed to be sequential. Two items with sequential positions can share the same rank."@en ;
  rdfs:label "rank"@en .

:eventCategory a owl:ObjectProperty ;
  rdfs:domain :AthleteEvent ;
  rdfs:range :AthleticEventCategory ;
  rdfs:comment "The category of events this athletic event belongs to."@en ;
  rdfs:label "event category" .

:siblingOrdering a owl:DatatypeProperty ;
	rdfs:domain owl:Thing ;
	rdfs:range xsd:integer ;
	rdfs:comment "The numeric order of an object among siblings of the same property or type."@en ;
	rdfs:label "sibling ordering"@en .

# widen the domain of sportEvent to include our AthleticEventRole
schema:sportsEvent rdfs:domain [
  rdf:type owl:Class ;
  owl:unionOf ( schema:ExerciseAction :AthleticEventRole );
] .

# add schema:competitor to our AthleticEventCompetitor role
schema:competitor rdfs:domain [
  rdf:type owl:Class ;
  owl:unionOf ( schema:SportsTeam :AthleticEventCompetitor )
] .

# NB: These are currently pending properties in schema.org. We will remove them 
# from here when they get integrated in a future version of schema.org.
schema:about a owl:ObjectProperty ;
  rdfs:domain schema:CreativeWork ;
  rdfs:range owl:Thing ;
  rdfs:comment "The subject matter of the content."@en ;
  rdfs:label "about"@en .

schema:subjectOf a owl:ObjectProperty ;
  rdfs:domain owl:Thing ;
  rdfs:range [
    rdf:type owl:Class ;
    owl:unionOf ( schema:CreativeWork schema:Event )
  ];
  rdfs:comment "A creative work or event about this thing."@en ;
  rdfs:label "subjectOf" .

##
## step count: note this is a virtual endpoint which is dynamically populated when requested
:steps a owl:DatatypeProperty;
  rdfs:comment "step counts for an individual.";
  rdfs:label "step counts for an individual.";
  rdfs:domain schema:Person;
  rdfs:range :StepAction
.

####
# Classes
####
:AggregateTeam a owl:Class ;
	rdfs:subClassOf schema:SportsTeam ;
	rdfs:comment "A team of athletes in an athletic event who each run the full race with their aggregate score determined by some specified procedure."@en ;
	rdfs:label "Aggregate team"@en .

:AthleteCohort a owl:Class ;
	rdfs:subClassOf schema:PeopleAudience ;
	rdfs:comment "A set of participants in an athletic event grouped together for the purpose of scoring. The groupings are often defined in terms of age and gender."@en ;
	rdfs:label "Athlete cohort"@en .

:AthleteResult a owl:Class ;
	rdfs:subClassOf schema:ListItem ;
	rdfs:comment "A ranking, within a particular athlete cohort, for an competitor who successfully completes an athletic event course or course segment."@en ;
	rdfs:label "Athlete result"@en .

:AthleteResultList a owl:Class ;
	rdfs:subClassOf schema:ItemList ;
	rdfs:comment "A ranked list of the results of an athletic event, usually bound to a particular athlete cohort."@en ;
	rdfs:label "Athlete result list"@en .

:AthleteTimingAction a owl:Class ;
	rdfs:subClassOf schema:CreateAction ;
	rdfs:comment "Observing and reporting the time and location of an athlete traversing an athletic event course. In the case of a normal RFID timed event, the agent is the timer, the object is the timing tag worn by the athlete, and the instrument is the timing device used to obtain the measurement. Those values will differ in other circumstances, say if the timing data is contained in a photograph taken by a spectator and uploaded during the race for the purpose of extracting the timing data."@en ;
	rdfs:label "Athlete timing action"@en .

:AthleteTimingController a owl:Class ;
	rdfs:subClassOf :AthleteTimingProduct ;
	rdfs:comment "An RFID timing controller used to process RFID tag reads during athlete events."@en ;
	rdfs:label "Athlete timing controller"@en .

:AthleteTimingProduct a owl:Class ;
	rdfs:subClassOf schema:Product ;
	rdfs:comment "An abstract class representing physical devices used for timing athletes."@en ;
	rdfs:label "Athlete timing product"@en .

:AthleteTimingSensor a owl:Class ;
	rdfs:subClassOf :AthleteTimingController ;
	rdfs:comment "The antenna deployed on an athletic course that actually senses the RFID timing tag in its RFID field. There will often be multiple sensors deployed that are associated with a given timing controller."@en ;
	rdfs:label "Athlete timing sensor"@en .

:AthleteTimingTag a owl:Class ;
	rdfs:subClassOf :AthleteTimingProduct ;
	rdfs:comment "An RFID athlete timing tag, usually contained in an athlete's bib."@en ;
	rdfs:label "Athlete timing tag"@en .

:AthleticCourse a owl:Class ;
	rdfs:subClassOf schema:Place ;
	rdfs:comment "A course on which an athletic event participant competes. This can refer to the entire course of an event, or a sub-course. A course is defined as the interval between two checkpoints."@en ;
	rdfs:label "Athletic course"@en .

:AthleticCourseCheckpoint a owl:Class ;
	rdfs:subClassOf :AthleticCourse ;
	rdfs:comment "A marked physical point within an athletic course which is used to mark a participant's progress along the course."@en ;
	rdfs:label "Athletic course checkpoint"@en .

:AthleticEvent a owl:Class ;
	rdfs:subClassOf schema:SportsEvent ;
	rdfs:comment "A sports event that occurs in one or more specific places at a definite time and comprises one or more athletic races."@en ;
	rdfs:label "Athletic event"@en .

:AthleticEventAction a owl:Class ;
  rdfs:subClassOf schema:ExerciseAction ;
  rdfs:comment "An exercise action performed during an athletic event."@en ;
  rdfs:label "Athletic event action"@en .

:AthleticEventBrand a owl:Class ;
	rdfs:subClassOf :AthleticEvent ;
	rdfs:comment "A collection of athletic events that form a unique brand. The individual events usually occur once per year, and the collection spans mutliple years. Also, the events are usually owned by a single organization that manages and cultivates the brand. Compare to an athletic event series."@en ;
	rdfs:label "Athletic event brand"@en .

:AthleticEventCompetitor a owl:Class ;
	rdfs:subClassOf :AthleticEventRole ;
	rdfs:comment "A role that an entry (such as a person or sports team) plays when they participate in an athletic event."@en ;
	rdfs:label "Athletic Event Competitor"@en .

:AthleticEventProduct a owl:Class ;
	rdfs:subClassOf schema:Product ;
	rdfs:comment "An product offered in the context of an athletic event."@en ;
	rdfs:label "Athletic event product"@en .

:AthleticEventRole a owl:Class ;
	rdfs:subClassOf schema:Role ;
	rdfs:comment "An abstract role that encompasses all roles around athletic events."@en ;
	rdfs:label "Athletic event role"@en .

:AthleticEventSeries a owl:Class ;
	rdfs:subClassOf :AthleticEvent ;
	rdfs:comment "A collection of athletic events, usually over the course of a single calendar year, that comprise a thematic sequence. Compare to an athletic event brand."@en ;
	rdfs:label "Athletic event series"@en .

:AthleticRace a owl:Class ;
	rdfs:subClassOf :AthleticEvent ;
	rdfs:comment "An athletic event where multiple people, participating either as individuals or in teams, compete over a closed course in one or more athletic disciplines."@en ;
	rdfs:label "Athletic race"@en .

:AggregateAthleticEventAction a owl:Class ;
  rdfs:subClassOf :AthleticEventAction ;
  rdfs:comment "A multi-course athletic event action that comprises multiple different exercise types."@en ;
	rdfs:label "Aggregate action"@en .

:BikeAction a owl:Class ;
	rdfs:subClassOf :AthleticEventAction ;
	rdfs:comment "Athletic event action by biking"@en ;
	rdfs:label "Bike Action"@en .

:CheckpointTimingDevice a owl:Class ;
	rdfs:subClassOf :AthleticEventRole ;
	rdfs:comment "A timing controller and sensors when deployed at a given checkpoint on a course."@en ;
	rdfs:label "Checkpoint timing device"@en .

:CrossCountryTeam a owl:Class ;
	rdfs:subClassOf :AggregateTeam ;
	rdfs:comment "An aggregate team in a cross-country style event."@en ;
	rdfs:label "Cross-country team"@en .

:LeaderBoard a owl:Class ;
	rdfs:subClassOf :AthleteResultList ;
	rdfs:comment "A short result list comprised of the current leaders of an athletic event. Often, this list is limited to a particular cohort of participants."@en ;
	rdfs:label "Leader board"@en .

:LegacyDataRecord a owl:Class ;
	rdfs:subClassOf schema:Intangible ;
	rdfs:comment "A legacy data record holds structured information from a legacy data system."@en ;
	rdfs:label "Legacy data record"@en .

:LegacyDataRole a owl:Class ;
	rdfs:subClassOf schema:Role ;
	rdfs:comment "A role played by a legacy data record in the context of some thing."@en ;
	rdfs:label "Legacy data role"@en .

:ObstacleAction a owl:Class ;
	rdfs:subClassOf :AthleticEventAction ;
	rdfs:comment "Athletic event action on an obstacle course"@en ;
	rdfs:label "Obstacle Action"@en .

:RacerMetrics a owl:Class ;
  rdfs:subClassOf schema:DataFeed;
  rdfs:comment "A set of data metrics for a given athlete. The about property should be used to refer to the athlete (schema:Person) about whom the metrics are computed."@en ;
  rdfs:label "Racer metrics"@en .

:RelayTeam a owl:Class ;
	rdfs:subClassOf schema:SportsTeam ;
	rdfs:comment "A team of athletes in an athletic event that each run part of the event course and their overall time is the sum of their individual times."@en ;
	rdfs:label "Relay team"@en .

:RunAction a owl:Class ;
	rdfs:subClassOf :AthleticEventAction ;
	rdfs:comment "Athletic event action by running"@en ;
	rdfs:label "Run Action"@en .

:SnowAction a owl:Class ;
	rdfs:subClassOf :AthleticEventAction ;
	rdfs:comment "Athletic event action in the snow."@en ;
	rdfs:label "Snow Action"@en .

:SnowShoeAction a owl:Class ;
	rdfs:subClassOf :SnowAction ;
	rdfs:comment "Athletic event action by snowshoeing."@en ;
	rdfs:label "Snowshoe Action"@en .

:StepAction a owl:Class ;
	rdfs:subClassOf :AthleticEventAction ;
	rdfs:comment "Athletic event action by stepping"@en ;
	rdfs:label "Step Action"@en .

:SwimAction a owl:Class ;
	rdfs:subClassOf :AthleticEventAction ;
	rdfs:comment "Athletic event action by swimming"@en ;
	rdfs:label "Swim Action"@en .

:AthleticEventCategory a owl:Class ;
	rdfs:subClassOf schema:Enumeration ;
	rdfs:comment "A type of athletic event, like marathon or triathlon."@en ;
	rdfs:label "Athletic event category"@en .

:AdventureEvent a owl:NamedIndividual , :AthleticEventCategory ;
  rdfs:label "Adventure Event"@en ;
	rdfs:comment "An adventure athletic event."@en .

:AquabikeEvent a owl:NamedIndividual , :AthleticEventCategory ;
  rdfs:comment "An athletic event comprised of swim and bike activities."@en ;
	rdfs:label "Aquabike Event"@en .

:AquathlonEvent a owl:NamedIndividual , :AthleticEventCategory ;
  rdfs:label "Aquathlon Event"@en ;
	rdfs:comment "An athletic event comprised of a swim and run."@en .

:CyclingEvent a owl:NamedIndividual , :AthleticEventCategory ;
  rdfs:label "Cycling Event"@en ;
	rdfs:comment "A cycling athletic event."@en .

:DuathlonEvent a owl:NamedIndividual , :AthleticEventCategory ;
  rdfs:label "Duathlon Event"@en ;
	rdfs:comment "An athletic event with two activities."@en .

:MountainBikeEvent a owl:NamedIndividual , :AthleticEventCategory ;
  rdfs:comment "A mountain biking athletic event."@en ;
	rdfs:label "Mountain Bike Event"@en .

:MultisportHalfIronmanEvent a owl:NamedIndividual , :AthleticEventCategory ;
  rdfs:label "Half Ironman Event"@en ;
	rdfs:comment "A half ironman athletic event."@en .

:MultisportIronManEvent a owl:NamedIndividual , :AthleticEventCategory ;
  rdfs:comment "An ironman athletic event."@en ;
	rdfs:label "Ironman Event"@en .

:MultisportOlympicEvent a owl:NamedIndividual , :AthleticEventCategory ;
  rdfs:comment "An olympic triathlon."@en ;
	rdfs:label "Olympic Triathlon Event"@en .

:MultisportSprintEvent a owl:NamedIndividual , :AthleticEventCategory ;
  rdfs:comment "A sprint triathlon."@en ;
	rdfs:label "Sprint Triathlon Event"@en .

:ObstacleEvent a owl:NamedIndividual , :AthleticEventCategory ;
  rdfs:comment "An obstacle athletic event."@en ;
	rdfs:label "Obstacle Event"@en .

:OtherEvent a owl:NamedIndividual , :AthleticEventCategory ;
  rdfs:comment "An athletic event in an unspecified category."@en ;
	rdfs:label "Other Event"@en .

:Run15kToHalfMarathonEvent a owl:NamedIndividual , :AthleticEventCategory ;
  rdfs:label "Run 15K to Half Marathon Event"@en ;
	rdfs:comment "A running event with a distance from 15K up to a half marathon."@en .

:Run5kTo15kEvent a owl:NamedIndividual , :AthleticEventCategory ;
  rdfs:comment "A running event from 5 to 15 kilometers in distance."@en ;
	rdfs:label "Run 5K to 15K"@en .

:RunHalfToFullMarathonEvent a owl:NamedIndividual , :AthleticEventCategory ;
  rdfs:label "Half to Full Marathon Event"@en ;
	rdfs:comment "A running event with a distance from a half to a full marathon."@en .

:RunMarathonEvent a owl:NamedIndividual , :AthleticEventCategory ;
  rdfs:comment "A marathon."@en ;
	rdfs:label "Marathon Event"@en .

:RunUltraEvent a owl:NamedIndividual , :AthleticEventCategory ;
  rdfs:comment "An ultra-marathon."@en ;
	rdfs:label "Ultramarathon Event"@en .

:RunUpTo5kEvent a owl:NamedIndividual , :AthleticEventCategory ;
  rdfs:label "Run up to 5K Event"@en ;
	rdfs:comment "A running event up to 5K in distance."@en .

:SnowEvent a owl:NamedIndividual , :AthleticEventCategory ;
  rdfs:comment "An athletic event in snow."@en ;
	rdfs:label "Snow Event"@en .

:SwimEvent a owl:NamedIndividual , :AthleticEventCategory ;
  rdfs:label "Swim Event"@en ;
	rdfs:comment "A swimming athletic event."@en .

# make subclasses disjoint
[] a owl:AllDifferent ;
	owl:members (
    :AdventureEvent
    :AquabikeEvent
    :AquathlonEvent
    :CyclingEvent
    :DuathlonEvent
    :MountainBikeEvent
    :MultisportHalfIronmanEvent
    :MultisportIronmanEvent
    :MultisportOlympicEvent 
    :MultisportSprintEvent 
    :ObstacleEvent
    :OtherEvent
    :Run15kToHalfMarathonEvent
    :Run5kTo15kEvent
    :RunHalfToFullMarathonEvent
    :RunMarathonEvent
    :RunUltraEvent
    :RunUpTo5kEvent
    :SnowEvent
    :SwimEvent
  ) .

[] a owl:AllDisjointClasses ;
	owl:members (
    :AthleticEventBrand
    :AthleticEventSeries
    :AthleticRace
  ) .

	


