@prefix : <http://adp.athlinks.com/schema/> .
@prefix dc: <http://purl.org/dc/elements/1.1/> .
@prefix owl: <http://www.w3.org/2002/07/owl#> .
@prefix rdf: <http://www.w3.org/1999/02/22-rdf-syntax-ns#> .
@prefix xml: <http://www.w3.org/XML/1998/namespace> .
@prefix xsd: <http://www.w3.org/2001/XMLSchema#> .
@prefix rdfs: <http://www.w3.org/2000/01/rdf-schema#> .
@prefix schema: <http://schema.org/> .
@base <http://adp.athlinks.com/schema> .

<http://adp.athlinks.com/schemax> rdf:type owl:Ontology; rdf:about "schema-latest-owl.ttl" .

<http://adp.athlinks.com/schema> rdf:type owl:Ontology ;
                                  owl:versionIRI : ;
                                  owl:imports <http://adp.athlinks.com/schemax> ;
                                  rdfs:comment "This file contains Athlinks data vocabulary. The vocabulary is based on the schema.org ontology with our own extensions for concepts specific to human endurance events."@en ;
                                  rdfs:label "Athlinks data vocabulary"@en ;
                                  dc:contributor "astn"^^xsd:string ,
                                                 "nextdude"^^xsd:string ,
                                                 "warren"^^xsd:string .

#################################################################
#    Annotation properties
#################################################################

###  http://purl.org/dc/elements/1.1/contributor
dc:contributor rdf:type owl:AnnotationProperty .


###  http://purl.org/dc/elements/1.1/creator
dc:creator rdf:type owl:AnnotationProperty .


###  http://purl.org/dc/elements/1.1/date
dc:date rdf:type owl:AnnotationProperty .


#################################################################
#    Object Properties
#################################################################

###  http://adp.athlinks.com/schema/exerciseType
:exerciseType rdf:type owl:ObjectProperty ;
              rdfs:domain schema:ExerciseAction ;
              rdfs:range :AthleticEventCategory ;
              dc:creator "nextdude"^^xsd:string ;
              dc:date "2017-07-26T14:00:17Z"^^xsd:dateTime .


###  http://adp.athlinks.com/schema/legacyData
:legacyData rdf:type owl:ObjectProperty ;
            rdfs:domain owl:Thing ;
            rdfs:range :LegacyDataRole ;
            rdfs:comment "A legacy data record belonging to another system that is related to this object."@en ;
            rdfs:label "legacy data"@en .


#################################################################
#    Data properties
#################################################################


### http://adp.athlinks.com/schema/age
:age rdf:type owl:DatatypeProperty ;
                 rdfs:domain schema:Person ;
                 rdfs:range xsd:integer ;
                 dc:creator "nextdude"^^xsd:string ;
                 dc:date "2017-08-09T22:22:47Z"^^xsd:dateTime ;
                 rdfs:comment "The age (in years) of a person."@en ;
                 rdfs:label "Age"@en .

###  http://adp.athlinks.com/schema/siblingOrdering
:siblingOrdering rdf:type owl:DatatypeProperty ;
                 rdfs:domain owl:Thing ;
                 rdfs:range xsd:integer ;
                 dc:creator "nextdude"^^xsd:string ;
                 dc:date "2017-07-26T14:18:47Z"^^xsd:dateTime ;
                 rdfs:comment "The numeric order of an object among siblings of the same property or type."@en ;
                 rdfs:label "Sibling Ordering"@en .

### TODO: should be remodeled
:participatedIn a owl:ObjectProperty ;
  rdfs:domain schema:Person ;
  rdfs:range :ActivityFeature ;
  rdfs:comment "An indication of a person participating in an ActivityFeature."@en ;
  rdfs:label "participated in"@en .

## TODO: should be remodeled
:numberOfRaces a owl:DatatypeProperty ;
  rdfs:domain schema:Person ;
  rdfs:range xsd:integer ;
  rdfs:comment "Number of races completed by an athlete."@en ;
  rdfs:label "Number of races"@en .

#################################################################
#    Classes
#################################################################

###  http://adp.athlinks.com/schema/AggregateTeam
:AggregateTeam rdf:type owl:Class ;
               rdfs:subClassOf schema:SportsTeam ;
               dc:creator "nextdude"^^xsd:string ;
               dc:date "2017-05-22T05:19:09Z"^^xsd:dateTime ;
               rdfs:comment "A team of athletes in an athletic event who each run the full race with their aggregate score determined by some specified procedure."@en ;
               rdfs:label "Aggregate team"@en .


###  http://adp.athlinks.com/schema/Athlete
:Athlete rdf:type owl:Class ;
         rdfs:subClassOf :AthleticEventRole ;
         dc:creator "nextdude"^^xsd:string ;
         dc:date "2017-05-22T06:00:00Z"^^xsd:dateTime ;
         rdfs:comment "A role that a person or sports team plays when they participate in an athletic event."@en ;
         rdfs:label "Athlete"@en .


###  http://adp.athlinks.com/schema/AthleteCohort
:AthleteCohort rdf:type owl:Class ;
               rdfs:subClassOf schema:PeopleAudience ;
               dc:creator "nextdude"^^xsd:string ;
               dc:date "2017-05-22T06:00:00Z"^^xsd:dateTime ;
               rdfs:comment "A set of participants in an athletic event grouped together for the purpose of scoring. The groupings are usually defined in terms of age, gender, etc."@en ;
               rdfs:label "Athlete cohort"@en .


###  http://adp.athlinks.com/schema/AthleteIdentifierAssignment
:AthleteIdentifierAssignment rdf:type owl:Class ;
                             rdfs:subClassOf :AthleticEventRole ;
                             dc:creator "nextdude"^^xsd:string ;
                             dc:date "2017-05-22T06:00:00Z"^^xsd:dateTime ;
                             rdfs:comment "Supports the assignment of identifiers to athletes in the context of a particular event. Examples of identifiers are bibs or timing tags."@en ;
                             rdfs:label "Athlete identifier assignment"@en .


###  http://adp.athlinks.com/schema/AthleteResult
:AthleteResult rdf:type owl:Class ;
               rdfs:subClassOf schema:ListItem ;
               dc:creator "nextdude"^^xsd:string ;
               dc:date "2017-05-22T06:00:00Z"^^xsd:dateTime ;
               rdfs:comment "A computed time and set of rankings for an athlete who successfully completes an athletic event course. The set of rankings are within the cohorts to which the athlete belongs."@en ;
               rdfs:label "Athlete result"@en .


###  http://adp.athlinks.com/schema/AthleteResultList
:AthleteResultList rdf:type owl:Class ;
                   rdfs:subClassOf schema:ItemList ;
                   dc:creator "nextdude"^^xsd:string ;
                   dc:date "2017-05-22T06:00:00Z"^^xsd:dateTime ;
                   rdfs:comment "A ranked list of the results of an athletic event, usually bound to a particular athlete cohort."@en ;
                   rdfs:label "Athlete result list"@en .


###  http://adp.athlinks.com/schema/AthleteTimingAction
:AthleteTimingAction rdf:type owl:Class ;
                     rdfs:subClassOf schema:CreateAction ;
                     dc:creator "nextdude"^^xsd:string ;
                     dc:date "2017-05-22T05:19:09Z"^^xsd:dateTime ;
                     rdfs:comment "Observing and reporting the time and location of an athlete traversing an athletic event course. In the case of a normal RFID timed event, the agent is the timer, the object is the timing tag worn by the athlete, and the instrument is the timing device used to obtain the measurement. Those values will differ in other circumstances, say if the timing data is contained in a photograph taken by a spectator and uploaded during the race for the purpose of extracting the timing data."@en ;
                     rdfs:label "Athlete timing action"@en .


###  http://adp.athlinks.com/schema/AthleteTimingController
:AthleteTimingController rdf:type owl:Class ;
                         rdfs:subClassOf :AthleteTimingProduct ;
                         dc:creator "nextdude"^^xsd:string ;
                         dc:date "2017-05-22T06:00:00Z"^^xsd:dateTime ;
                         rdfs:comment "An RFID timing controller used to process RFID tag reads during athlete events."@en ;
                         rdfs:label "Athlete timing controller"@en .


###  http://adp.athlinks.com/schema/AthleteTimingProduct
:AthleteTimingProduct rdf:type owl:Class ;
                      rdfs:subClassOf schema:Product ;
                      dc:creator "nextdude"^^xsd:string ;
                      dc:date "2017-05-22T06:00:00Z"^^xsd:dateTime ;
                      rdfs:comment "An abstract class representing physical devices used for timing athletes."@en ;
                      rdfs:label "Athlete timing product"@en .


###  http://adp.athlinks.com/schema/AthleteTimingSensor
:AthleteTimingSensor rdf:type owl:Class ;
                     rdfs:subClassOf :AthleteTimingController ;
                     dc:creator "nextdude"^^xsd:string ;
                     dc:date "2017-05-22T06:00:00Z"^^xsd:dateTime ;
                     rdfs:comment "The antenna deployed on an athletic course that actually senses the RFID timing tag in its RFID field. There will often be multiple sensors deployed that are associated with a given timing controller."@en ;
                     rdfs:label "Athlete timing sensor"@en .


###  http://adp.athlinks.com/schema/AthleteTimingTag
:AthleteTimingTag rdf:type owl:Class ;
                  rdfs:subClassOf :AthleteTimingProduct ;
                  dc:creator "nextdude"^^xsd:string ;
                  dc:date "2017-05-22T06:00:00Z"^^xsd:dateTime ;
                  rdfs:comment "An RFID athlete timing tag, usually contained in an athlete's bib."@en ;
                  rdfs:label "Athlete timing tag"@en .


###  http://adp.athlinks.com/schema/AthleticCourse
:AthleticCourse rdf:type owl:Class ;
                rdfs:subClassOf schema:Place ;
                dc:creator "nextdude"^^xsd:string ;
                dc:date "2017-05-22T06:00:00Z"^^xsd:dateTime ;
                rdfs:comment "A course on which an athletic event participant competes. This can refer to the entire course of an event, or a sub-course. A course is defined as the interval between two checkpoints."@en ;
                rdfs:label "Athletic course"@en .


###  http://adp.athlinks.com/schema/AthleticCourseCheckpoint
:AthleticCourseCheckpoint rdf:type owl:Class ;
                          rdfs:subClassOf :AthleticCourse ;
                          dc:creator "nextdude"^^xsd:string ;
                          dc:date "2017-05-22T06:00:00Z"^^xsd:dateTime ;
                          rdfs:comment "A marked physical point within an athletic course which is used to mark a participant's progress along the course."@en ;
                          rdfs:label "Athletic course checkpoint"@en .


###  http://adp.athlinks.com/schema/AthleticEvent
:AthleticEvent rdf:type owl:Class ;
               rdfs:subClassOf schema:SportsEvent ;
               dc:creator "nextdude"^^xsd:string ;
               dc:date "2017-05-22T06:00:00Z"^^xsd:dateTime ;
               rdfs:comment "A sports event where multiple people, participating either as individuals or in teams, compete over a closed course in one or more athletic disciplines."@en ;
               rdfs:label "Athletic event"@en .


###  http://adp.athlinks.com/schema/AthleticEventBrand
:AthleticEventBrand rdf:type owl:Class ;
                    rdfs:subClassOf :AthleticEvent ;
                    owl:disjointWith :AthleticEventSeries ;
                    dc:creator "nextdude"^^xsd:string ;
                    dc:date "2017-06-27T02:51:03Z"^^xsd:dateTime ;
                    rdfs:comment "A collection of athletic events that form a unique brand. The individual events usually occur once per year, and the collection spans mutliple years. Also, the events are usually owned by a single organization that manages and cultivates the brand. Compare to an athletic event series."@en ;
                    rdfs:label "Athletic event brand"@en .


###  http://adp.athlinks.com/schema/AthleticEventCategory
:AthleticEventCategory rdf:type owl:Class ;
                       rdfs:subClassOf schema:Enumeration ;
                       dc:creator "nextdude"^^xsd:string ;
                       dc:date "2017-05-22T06:00:00Z"^^xsd:dateTime ;
                       rdfs:comment "A kind of athletic event."@en ;
                       rdfs:label "Athletic event category"@en .


###  http://adp.athlinks.com/schema/AthleticEventProduct
:AthleticEventProduct rdf:type owl:Class ;
                      rdfs:subClassOf schema:Product ;
                      dc:creator "nextdude"^^xsd:string ;
                      dc:date "2017-05-22T06:00:00Z"^^xsd:dateTime ;
                      rdfs:comment "An product offered in the context of an athletic event."@en ;
                      rdfs:label "Athletic event product"@en .


###  http://adp.athlinks.com/schema/AthleticEventRole
:AthleticEventRole rdf:type owl:Class ;
                   rdfs:subClassOf schema:Role ;
                   dc:creator "nextdude"^^xsd:string ;
                   dc:date "2017-05-22T06:00:00Z"^^xsd:dateTime ;
                   rdfs:comment "An abstract role that encompasses all roles around athletic events."@en ;
                   rdfs:label "Athletic event role"@en .

###  https://adp.athlinks.com/schema/AthleticEventEntry
:AthleticEventEntry rdf:type owl:Class ;
                    rdfs:subClassOf athlinks:AthleticEventRole ;
                    dc:creator "berg"^^xsd:string ;
                    dc:date "2017-09-12T12:00:00Z"^^xsd:dateTime ;
                    rdfs:comment "A concrete role that captures a Person's entry in an athletic event"

###  http://adp.athlinks.com/schema/AthleticEventSeries
:AthleticEventSeries rdf:type owl:Class ;
                     rdfs:subClassOf :AthleticEvent ;
                     dc:creator "nextdude"^^xsd:string ;
                     dc:date "2017-06-27T02:51:03Z"^^xsd:dateTime ;
                     rdfs:comment "A collection of athletic events, usually over the course of a single calendar year, that comprise a thematic sequence. Compare to an athletic event brand."@en ;
                     rdfs:label "Athletic event series"@en .


###  http://adp.athlinks.com/schema/BikeAction
:BikeAction rdf:type owl:Class ;
            rdfs:subClassOf schema:ExerciseAction ;
            dc:creator "nextdude"^^xsd:string ;
            dc:date "2017-07-26T14:07:23Z"^^xsd:dateTime ;
            rdfs:comment "Exercise by biking"@en ;
            rdfs:label "Bike Action"@en .


###  http://adp.athlinks.com/schema/CheckpointTimingDevice
:CheckpointTimingDevice rdf:type owl:Class ;
                        rdfs:subClassOf :AthleticEventRole ;
                        dc:creator "nextdude"^^xsd:string ;
                        dc:date "2017-05-22T06:00:00Z"^^xsd:dateTime ;
                        rdfs:comment "A timing controller and sensors when deployed at a given checkpoint on a course."@en ;
                        rdfs:label "Checkpoint timing device"@en .


###  http://adp.athlinks.com/schema/CrossCountryTeam
:CrossCountryTeam rdf:type owl:Class ;
                  rdfs:subClassOf :AggregateTeam ;
                  dc:creator "nextdude"^^xsd:string ;
                  dc:date "2017-05-22T05:21:23Z"^^xsd:dateTime ;
                  rdfs:comment "An aggregate team in a cross-country style event."@en ;
                  rdfs:label "Cross-country team"@en .


###  http://adp.athlinks.com/schema/LeaderBoard
:LeaderBoard rdf:type owl:Class ;
             rdfs:subClassOf :AthleteResultList ;
             rdfs:comment "A short result list comprised of the current leaders of an athletic event. Often, this list is limited to a particular cohort of participants."@en ;
             rdfs:label "Leader board"@en .


###  http://adp.athlinks.com/schema/LegacyDataRecord
:LegacyDataRecord rdf:type owl:Class ;
                  rdfs:subClassOf schema:Intangible ;
                  dc:creator "nextdude"^^xsd:string ;
                  dc:date "2017-05-22T06:00:00Z"^^xsd:dateTime ;
                  rdfs:comment "A legacy data record holds structured information from a legacy data system."@en ;
                  rdfs:label "Legacy data record"@en .


###  http://adp.athlinks.com/schema/LegacyDataRole
:LegacyDataRole rdf:type owl:Class ;
                rdfs:subClassOf schema:Role ;
                dc:creator "nextdude"^^xsd:string ;
                dc:date "2017-05-22T06:00:00Z"^^xsd:dateTime ;
                rdfs:comment "A role played by a legacy data record in the context of some thing."@en ;
                rdfs:label "Legacy data role"@en .


###  http://adp.athlinks.com/schema/ObstacleAction
:ObstacleAction rdf:type owl:Class ;
                rdfs:subClassOf schema:ExerciseAction ;
                dc:creator "nextdude"^^xsd:string ;
                dc:date "2017-07-26T14:16:41Z"^^xsd:dateTime ;
                rdfs:comment "Exercise on an obstacle course"@en ;
                rdfs:label "Obstacle Action"@en .


###  http://adp.athlinks.com/schema/RelayTeam
:RelayTeam rdf:type owl:Class ;
           rdfs:subClassOf schema:SportsTeam ;
           dc:creator "nextdude"^^xsd:string ;
           dc:date "2017-05-22T05:16:50Z"^^xsd:dateTime ;
           rdfs:comment "A team of athletes in an athletic event that each run part of the event course and their overall time is the sum of their individual times."@en ;
           rdfs:label "Relay team"@en .


###  http://adp.athlinks.com/schema/RunAction
:RunAction rdf:type owl:Class ;
           rdfs:subClassOf schema:ExerciseAction ;
           dc:creator "nextdude"^^xsd:string ;
           dc:date "2017-07-26T14:06:45Z"^^xsd:dateTime ;
           rdfs:comment "Exercise by running"@en ;
           rdfs:label "Run Action"@en .


###  http://adp.athlinks.com/schema/SwimAction
:SwimAction rdf:type owl:Class ;
            rdfs:subClassOf schema:ExerciseAction ;
            dc:creator "nextdude"^^xsd:string ;
            dc:date "2017-07-26T14:06:57Z"^^xsd:dateTime ;
            rdfs:comment "Exercise by swimming"@en ;
            rdfs:label "Swim Action"@en .


###  http://schema.org/GenderType
schema:GenderType dc:creator "nextdude"^^xsd:string ;
                  dc:date "2017-05-22T06:00:00Z"^^xsd:dateTime .

### TODO: This should be removed and we should use schema:Action
:ActivityFeature
  a owl:Class ;
  rdfs:subClassOf schema:QualitativeValue ;
  rdfs:comment "Flag describing an activity"@en ;
  rdfs:label "ActivityFeature"@en .

#################################################################
#    Individuals
#################################################################

:RunUpTo5k              a owl:NamedIndividual, :ActivityFeature ;
                        rdfs:comment "Instance of a flag indicating activity in a running event up to 5k in distance" ;
                        rdfs:label "Run up to 5k" .
:Run5kTo15k             a owl:NamedIndividual, :ActivityFeature ;
                        rdfs:comment "Instance of a flag indicating activity in a running event from 5k to 15k in distance" ;
                        rdfs:label "Run 5k to 15k" .
:Run15kToHalfMarathon   a owl:NamedIndividual, :ActivityFeature ;
                        rdfs:comment "Instance of a flag indicating activity in a running event from 15k to Half Marathon in distance" ;
                        rdfs:label "Run 15k to Half Marathon" .
:RunHalfToFullMarathon  a owl:NamedIndividual, :ActivityFeature ;
                        rdfs:comment "Instance of a flag indicating activity in a running event from Half Marathon to Full Marathon in distance" ;
                        rdfs:label "Run Half Marathon to Marathon" .
:RunMarathon            a owl:NamedIndividual, :ActivityFeature ;
                        rdfs:comment "Instance of a flag indicating activity in a Marathon running event" ;
                        rdfs:label "Run Marathon" .
:RunUltra               a owl:NamedIndividual, :ActivityFeature ;
                        rdfs:comment "Instance of a flag indicating activity in a Ultra-marathon running event" ;
                        rdfs:label "Run Ultra" .
:MultisportSprint       a owl:NamedIndividual, :ActivityFeature ;
                        rdfs:comment "Instance of a flag indicating activity in a Triathlon Sprint athletic event" ;
                        rdfs:label "Sprint Triathlon" .
:MultisportOlympic      a owl:NamedIndividual, :ActivityFeature ;
                        rdfs:comment "Instance of a flag indicating activity in a Triathlon Olympic athletic event" ;
                        rdfs:label "Olympic Triathlon" .
:MultisportHalfIronman  a owl:NamedIndividual, :ActivityFeature ;
                        rdfs:comment "Instance of a flag indicating activity in a Half Ironman athletic event" ;
                        rdfs:label "Half Ironman" .
:MultisportIronMan      a owl:NamedIndividual, :ActivityFeature ;
                        rdfs:comment "Instance of a flag indicating activity in an Ironman athletic event" ;
                        rdfs:label "Ironman" .
:Aquathlon              a owl:NamedIndividual, :ActivityFeature ;
                        rdfs:comment "Instance of a flag indicating activity in an Aquathlon athletic event" ;
                        rdfs:label "Aquathlon" .
:Aquabike               a owl:NamedIndividual, :ActivityFeature ;
                        rdfs:comment "Instance of a flag indicating activity in an Aquabike athletic event" ;
                        rdfs:label "Aquabike" .
:Duathlon               a owl:NamedIndividual, :ActivityFeature ;
                        rdfs:comment "Instance of a flag indicating activity in a Duathlon athletic event" ;
                        rdfs:label "Duathlon" .
:Swim                   a owl:NamedIndividual, :ActivityFeature ;
                        rdfs:comment "Instance of a flag indicating activity in a Swimming athletic event" ;
                        rdfs:label "Swim" .
:MountainBike           a owl:NamedIndividual, :ActivityFeature ;
                        rdfs:comment "Instance of a flag indicating activity in a Mountain Bike athletic event" ;
                        rdfs:label "Mountain Bike" .
:Cycling                a owl:NamedIndividual, :ActivityFeature ;
                        rdfs:comment "Instance of a flag indicating activity in a Cycling athletic event" ;
                        rdfs:label "Cycling" .
:Snow                   a owl:NamedIndividual, :ActivityFeature ;
                        rdfs:comment "Instance of a flag indicating activity in a Snowshow Running athletic event" ;
                        rdfs:label "Snowshow Running" .
:Adventure              a owl:NamedIndividual, :ActivityFeature ;
                        rdfs:comment "Instance of a flag indicating activity in an Adventure athletic event" ;
                        rdfs:label "Adventure" .
:Obstacle               a owl:NamedIndividual, :ActivityFeature ;
                        rdfs:comment "Instance of a flag indicating activity in an Obstacle Course athletic event" ;
                        rdfs:label "Obstacle" .
:Other                  a owl:NamedIndividual, :ActivityFeature ;
                        rdfs:comment "Instance of a flag indicating activity in an athletic event not described" ;
                        rdfs:label "Other" .

#################################################################
#    General axioms
#################################################################

[ rdf:type owl:AllDisjointClasses ;
  owl:members ( 
                :RunUpTo5k
                :Run5kTo15k
                :Run15kToHalfMarathon
                :RunHalfToFullMarathon
                :RunMarathon
                :RunUltra
                :MultisportSprint
                :MultisportOlympic
                :MultisportHalfIronman
                :MultisportIronMan
                :Aquathlon
                :Aquabike
                :Duathlon
                :Swim
                :MountainBike
                :Cycling
                :Snow
                :Adventure
                :Obstacle
                :Other
              )
] .

## Properties/Predicates

### http://adp.athlinks.com/schema/hasEntry
:hasEntry a owl:ObjectProperty ;
  rdfs:domain schema:Person ;
  rdfs:range athlinks:AthleticEventEntry .

### http://adp.athlinks.com/schema/entryBelongsTo
:entryBelongsTo a owl:ObjectProperty ;
  rdfs:domain athlinks:AthleticEventEntry ;
  rdfs:range athlinks:AthleticEvent .